Updates from Overleaf

PTR.v
@@ -1,658 +1,641 @@
+(*
+  Pointer Analysis for TAC IR
+*)
+
 From Coq Require Import String List Bool Arith ZArith PeanoNat.
-From Coq Require Import Sets.Ensembles.
 From Coq Require Import FSets FSetWeakList FMaps FMapWeakList.
 From Coq Require Import Relations DecidableType.
 Import ListNotations.
 
-(* ===== Import TAC Definitions ===== *)
-(* We assume TAC module is available with these definitions *)
-Module TAC.
-  Definition StackVar := nat.
-  
-  Inductive FieldKey :=
-  | FKPos  : nat -> FieldKey
-  | FKName : string -> FieldKey
-  | FKBoth : nat -> string -> FieldKey.
-  
-  Inductive ConstV : Type :=
-  | KInt      : Z -> ConstV
-  | KBool     : bool -> ConstV
-  | KString   : string -> ConstV
-  | KNone     : ConstV
-  | KStopIter : ConstV.
-  
-  Inductive Instruction : Type :=
-  | IMov          : StackVar -> StackVar -> Instruction
-  | ILoadConst    : StackVar -> ConstV -> Instruction
-  | ILoadLocal    : StackVar -> string -> Instruction
-  | ILoadGlobal   : StackVar -> string -> Instruction
-  | ISetLocal     : string -> StackVar -> Instruction
-  | ILookupDunderUnary  : StackVar -> string -> StackVar -> Instruction
-  | ILookupDunderBinary : StackVar -> string -> StackVar -> StackVar -> Instruction
-  | IResolveOverload    : StackVar -> StackVar -> StackVar -> StackVar -> Instruction
-  | IGetAttr      : StackVar -> StackVar -> string -> Instruction
-  | ISetAttr      : StackVar -> string -> StackVar -> Instruction
-  | IUnpack       : list StackVar -> StackVar -> Instruction
-  | IConstructTuple : StackVar -> list StackVar -> Instruction
-  | IConstructDict  : StackVar -> list (StackVar * StackVar) -> Instruction
-  | IBind         : StackVar -> StackVar -> StackVar -> StackVar -> Instruction
-  | ICall         : StackVar -> StackVar -> Instruction
-  | IAssumeValue  : StackVar -> ConstV -> Instruction
-  | IExit         : Instruction.
-End TAC.
+Set Implicit Arguments.
 
 Import TAC.
 
-(* ===== Abstract Objects ===== *)
-Module AbstractObject.
-  Inductive t :=
-  | Loc      : nat -> nat -> t           (* allocation site: (block, instr) *)
-  | Param    : string -> t               (* external parameter *)
-  | Imm      : ConstV -> t               (* immutable constant *)
-  | Locals   : t                         (* local variables root *)
-  | Globals  : t                         (* global variables root *)
-  | Temp     : t                         (* stack temporaries root *)
-  | RetUp    : t.                        (* summary return object *)
-  
-  Definition eq_dec : forall x y : t, {x = y} + {x <> y}.
-  Proof.
-    decide equality; try decide equality.
-    - apply Nat.eq_dec.
-    - apply Nat.eq_dec.
-    - apply String.string_dec.
-    - apply Z.eq_dec.
-    - apply Bool.bool_dec.
-    - apply String.string_dec.
-  Defined.
-End AbstractObject.
+Module PointerAnalysis.
 
-(* ===== Field Keys ===== *)
-Module AbstractField.
-  Definition t := FieldKey.
-  
-  Definition star : t := FKName "*".        (* wildcard field *)
-  Definition args : t := FKName "args".     (* for bound callables *)
-  Definition kwargs : t := FKName "kwargs". (* for bound callables *)
-  
-  Definition eq_dec : forall x y : t, {x = y} + {x <> y}.
-  Proof.
-    decide equality; try decide equality.
-    - apply Nat.eq_dec.
-    - apply String.string_dec.
-    - apply Nat.eq_dec.
-    - apply String.string_dec.
-  Defined.
-  
-  (* Check if a field key matches (with wildcard support) *)
-  Definition matches (k1 k2 : t) : bool :=
-    match k1, k2 with
-    | FKPos n1, FKPos n2 => Nat.eqb n1 n2
-    | FKName s1, FKName s2 => String.eqb s1 s2
-    | FKBoth n1 s1, FKBoth n2 s2 => andb (Nat.eqb n1 n2) (String.eqb s1 s2)
-    | FKPos n, FKBoth n' _ => Nat.eqb n n'
-    | FKName s, FKBoth _ s' => String.eqb s s'
-    | FKBoth n' _, FKPos n => Nat.eqb n n'
-    | FKBoth _ s', FKName s => String.eqb s s'
-    | _, _ => false
-    end.
-End AbstractField.
+  (* ===== Abstract Objects ===== *)
+  Module AbstractObject.
+    Inductive t :=
+    | Location : nat -> nat -> t           (* allocation site: (block, instr) *)
+    | Param    : option string -> t        (* parameter with optional name *)
+    | ImmType  : nat -> t                  (* immutable by type hash *)
+    | ImmConst : ConstV -> t               (* immutable constant value *)
+    | Locals   : t                         (* locals scope *)
+    | Globals  : t.                        (* globals scope *)
+    
+    Definition eq_dec : forall x y : t, {x = y} + {x <> y}.
+    Proof.
+      decide equality; try apply Nat.eq_dec; try apply String.string_dec.
+      - decide equality; apply String.string_dec.
+      - destruct c, c0; try discriminate; try (left; reflexivity);
+        try (right; discriminate); 
+        try (decide equality; [apply Z.eq_dec | apply Bool.bool_dec | apply String.string_dec]).
+    Defined.
+  End AbstractObject.
 
-(* ===== Type System Interface ===== *)
-Module Type TypeSystemInterface.
-  Import AbstractObject.
-  Import AbstractField.
-  
-  (* Abstract type expressions *)
-  Parameter TypeExpr : Type.
-  Parameter type_bot : TypeExpr.
-  Parameter type_top : TypeExpr.
-  Parameter type_join : TypeExpr -> TypeExpr -> TypeExpr.
-  Parameter type_meet : TypeExpr -> TypeExpr -> TypeExpr.
-  Parameter type_leq : TypeExpr -> TypeExpr -> bool.
-  
-  (* Effect summaries for callables *)
-  Record EffectSummary := {
-    eff_new : bool;                    (* allocates new object *)
-    eff_update : list (nat * t);       (* updated fields: (param_idx, field) pairs *)
-    eff_points_to_args : bool;         (* result may alias arguments *)
-  }.
-  
-  (* Default effect: pure function *)
-  Parameter default_effect : EffectSummary.
-  
-  (* Get effect summary for a callable object *)
-  Parameter get_callable_effect : AbstractObject.t -> option EffectSummary.
-  
-  (* Get type of an abstract object *)
-  Parameter object_type : AbstractObject.t -> TypeExpr.
-  
-  (* Type of allocation based on instruction *)
-  Parameter alloc_type : Instruction -> TypeExpr.
-End TypeSystemInterface.
+  (* ===== Type System Interface ===== *)
+  Module Type TypeSystemSig.
+    Import AbstractObject.
+    
+    Parameter TypeExpr : Type.
+    Parameter type_bot : TypeExpr.
+    Parameter type_top : TypeExpr.
+    Parameter type_join : TypeExpr -> TypeExpr -> TypeExpr.
+    Parameter type_is_subtype : TypeExpr -> TypeExpr -> bool.
+    Parameter type_is_immutable : TypeExpr -> bool.
+    
+    (* Side effects *)
+    Record SideEffect := {
+      se_new : bool;
+      se_bound_method : bool;
+      se_update : option TypeExpr;
+      se_update_indices : list nat;
+      se_points_to_args : bool
+    }.
+    
+    Parameter empty_effect : SideEffect.
+    
+    (* Type operations *)
+    Parameter literal_type : ConstV -> TypeExpr.
+    Parameter get_type_hash : TypeExpr -> nat.
+    
+    (* Overloaded function handling *)
+    Parameter is_overloaded : TypeExpr -> bool.
+    Parameter is_property : TypeExpr -> bool.
+    Parameter is_bound_method : TypeExpr -> bool.
+    Parameter any_new : TypeExpr -> bool.
+    Parameter all_new : TypeExpr -> bool.
+    Parameter get_return : TypeExpr -> TypeExpr.
+    Parameter get_side_effect : TypeExpr -> SideEffect.
+    
+    (* Module/class member access *)
+    Parameter subscr : TypeExpr -> string -> TypeExpr.
+    Parameter subscr_literal : TypeExpr -> ConstV -> TypeExpr.
+    Parameter subscr_index : TypeExpr -> nat -> TypeExpr.
+    
+    (* Function application *)
+    Parameter partial : TypeExpr -> list TypeExpr -> TypeExpr.
+    Parameter get_unop : TypeExpr -> string -> TypeExpr.
+    Parameter partial_binop : TypeExpr -> TypeExpr -> string -> TypeExpr.
+    
+    (* Type constructors *)
+    Parameter make_list_constructor : TypeExpr.
+    Parameter make_tuple_constructor : TypeExpr.
+    Parameter make_dict_constructor : TypeExpr.
+    Parameter make_set_constructor : TypeExpr.
+    Parameter make_slice_constructor : TypeExpr.
+    
+    (* Checks *)
+    Parameter type_is_callable : TypeExpr -> bool.
+  End TypeSystemSig.
 
-(* ===== Main Analysis Module ===== *)
-Module PointerAnalysis (TS : TypeSystemInterface).
-  Import TS.
-  Import AbstractObject.
-  Import AbstractField.
-  
-  (* ===== Object Sets using FSets ===== *)
-  Module AODec <: DecidableType.
-    Definition t := AbstractObject.t.
-    Definition eq := @eq t.
-    Definition eq_refl := @eq_refl t.
-    Definition eq_sym := @eq_sym t.
-    Definition eq_trans := @eq_trans t.
-    Definition eq_dec := AbstractObject.eq_dec.
-  End AODec.
-  
-  Module ObjectSet := FSetWeakList.Make(AODec).
-  
-  (* ===== Points-to Domain ===== *)
-  Module AOMap := FMapWeakList.Make(AODec).
-  Module AFMap := FMapWeakList.Make(AbstractField).
-  
-  Definition FieldMap := AFMap.t ObjectSet.t.
-  Definition PointsTo := AOMap.t FieldMap.
-  
-  Definition empty_points_to : PointsTo := AOMap.empty FieldMap.
-  
-  (* Lookup with proper handling of empty cases *)
-  Definition points_to_lookup (P : PointsTo) (o : AbstractObject.t) (f : AbstractField.t) : ObjectSet.t :=
-    match AOMap.find o P with
-    | Some fm => 
-        match AFMap.find f fm with
-        | Some objs => objs
-        | None => ObjectSet.empty
-        end
-    | None => ObjectSet.empty
-    end.
-  
-  (* Points-to update with proper field map handling *)
-  Definition points_to_update (P : PointsTo) (o : AbstractObject.t) (f : AbstractField.t) 
+  Module Analysis (TS : TypeSystemSig).
+    Import TS AbstractObject.
+    
+    (* ===== Core Domains ===== *)
+    Module AODec <: DecidableType.
+      Definition t := AbstractObject.t.
+      Definition eq := @eq t.
+      Definition eq_refl := @eq_refl t.
+      Definition eq_sym := @eq_sym t.
+      Definition eq_trans := @eq_trans t.
+      Definition eq_dec := AbstractObject.eq_dec.
+    End AODec.
+    
+    Module ObjectSet := FSetWeakList.Make(AODec).
+    Module AOMap := FMapWeakList.Make(AODec).
+    
+    Module FKDec <: DecidableType.
+      Definition t := FieldKey.
+      Definition eq := @eq t.
+      Definition eq_refl := @eq_refl t.
+      Definition eq_sym := @eq_sym t.
+      Definition eq_trans := @eq_trans t.
+      Definition eq_dec : forall x y : t, {x = y} + {x <> y}.
+      Proof.
+        decide equality; try apply Nat.eq_dec; try apply String.string_dec.
+      Defined.
+    End FKDec.
+    
+    Module FieldMap := FMapWeakList.Make(FKDec).
+    
+    Definition PointsTo := AOMap.t (FieldMap.t ObjectSet.t).
+    Definition TypeMap := AOMap.t TypeExpr.
+    Definition DirtyMap := AOMap.t (FieldMap.t bool).
+    Definition StackEnv := StackVar -> ObjectSet.t.
+    Definition ProgramPoint := (nat * nat)%type.
+    
+    (* ===== Field Key Helpers ===== *)
+    
+    Definition wildcard : FieldKey := FKName "*".
+    Definition self_field : FieldKey := FKName "self".
+    Definition func_field : FieldKey := FKName "__func__".
+    Definition args_field : FieldKey := FKName "args".
+    Definition kwargs_field : FieldKey := FKName "kwargs".
+    
+    (* Field key subsumption *)
+    Definition is_star (k:FieldKey) : bool :=
+      match k with | FKName s => String.eqb s "*" | _ => false end.
+    
+    Definition field_matches (k1 k2 : FieldKey) : bool :=
+      if orb (is_star k1) (is_star k2) then true else
+      match k1, k2 with
+      | FKPos n1,  FKPos n2  => Nat.eqb n1 n2
+      | FKName s1, FKName s2 => String.eqb s1 s2
+      | FKBoth n1 s1, FKBoth n2 s2 => Nat.eqb n1 n2 && String.eqb s1 s2
+      | FKPos n,   FKBoth n' _ | FKBoth n' _, FKPos n   => Nat.eqb n n'
+      | FKName s,  FKBoth _ s' | FKBoth _ s', FKName s  => String.eqb s s'
+      | _, _ => false
+      end.
+    
+    (* ===== Empty/Initial Values ===== *)
+    
+    Definition empty_points_to : PointsTo := AOMap.empty _.
+    Definition empty_type_map : TypeMap := AOMap.empty _.
+    Definition empty_dirty_map : DirtyMap := AOMap.empty _.
+    Definition empty_stack : StackEnv := fun _ => ObjectSet.empty.
+    
+    (* Get immutable object for constant value *)
+    Definition immutable_const (c : ConstV) : ObjectSet.t :=
+      ObjectSet.singleton (ImmConst c).
+    
+    (* Get immutable object for type (coarse) *)
+    Definition immutable_type (ty : TypeExpr) : ObjectSet.t :=
+      ObjectSet.singleton (ImmType (get_type_hash ty)).
+    
+    (* ===== Points-to operations with subsumption ===== *)
+    
+    Definition points_to_lookup (P : PointsTo) (o : AbstractObject.t) (f : FieldKey) : ObjectSet.t :=
+      match AOMap.find o P with
+      | Some fm =>
+          FieldMap.fold (fun k objs acc =>
+            if field_matches k f || field_matches f k then 
+              ObjectSet.union acc objs 
+            else acc
+          ) fm ObjectSet.empty
+      | None => ObjectSet.empty
+      end.
+    
+    Definition points_to_update (P : PointsTo) (o : AbstractObject.t) (f : FieldKey)
                                (objs : ObjectSet.t) : PointsTo :=
-    let fm := match AOMap.find o P with
-             | Some fm => fm
-             | None => AFMap.empty ObjectSet.t
-             end in
-    let fm' := AFMap.add f objs fm in
-    AOMap.add o fm' P.
-  
-  (* Weak/Strong update based on target set size *)
-  Definition upd_points_to (P : PointsTo) (targets : ObjectSet.t) (f : AbstractField.t) 
-                           (new_objs : ObjectSet.t) : PointsTo :=
-    if ObjectSet.cardinal targets =? 1
-    then 
-      (* Strong update *)
-      match ObjectSet.choose targets with
-      | Some tgt => points_to_update P tgt f new_objs
-      | None => P  (* shouldn't happen *)
-      end
-    else
-      (* Weak update *)
-      ObjectSet.fold (fun tgt P' =>
-        let old := points_to_lookup P' tgt f in
-        points_to_update P' tgt f (ObjectSet.union old new_objs)
-      ) targets P.
-  
-  (* ===== Type Domain ===== *)
-  Definition TypeMap := AOMap.t TypeExpr.
-  
-  Definition empty_type_map : TypeMap := AOMap.empty TypeExpr.
-  
-  Definition type_lookup (T : TypeMap) (o : AbstractObject.t) : TypeExpr :=
-    match AOMap.find o T with
-    | Some ty => ty
-    | None => type_bot
-    end.
-  
-  Definition type_update (T : TypeMap) (o : AbstractObject.t) (ty : TypeExpr) : TypeMap :=
-    let old_ty := type_lookup T o in
-    AOMap.add o (type_join old_ty ty) T.
-  
-  (* ===== Abstract State ===== *)
-  Record AbstractState := {
-    as_points_to : PointsTo;
-    as_types : TypeMap;
-    (* Dirty domain omitted for now *)
-  }.
-  
-  Definition empty_state : AbstractState := {|
-    as_points_to := empty_points_to;
-    as_types := empty_type_map;
-  |}.
-  
-  (* ===== Stack Environment ===== *)
-  Definition StackEnv := StackVar -> ObjectSet.t.
-  
-  Definition empty_stack : StackEnv := fun _ => ObjectSet.empty.
-  
-  Definition stack_lookup (S : StackEnv) (v : StackVar) : ObjectSet.t := S v.
-  
-  Definition stack_update (S : StackEnv) (v : StackVar) (objs : ObjectSet.t) : StackEnv :=
-    fun v' => if Nat.eq_dec v v' then objs else S v'.
-  
-  (* ===== Combined State ===== *)
-  Record State := {
-    st_abstract : AbstractState;
-    st_stack : StackEnv;
-  }.
-  
-  Definition empty_combined_state : State := {|
-    st_abstract := empty_state;
-    st_stack := empty_stack;
-  |}.
-  
-  (* ===== Helper Functions ===== *)
-  
-  (* Program point *)
-  Definition ProgramPoint := (nat * nat)%type.
-  
-  (* Create allocation site from program point *)
-  Definition alloc_site (pp : ProgramPoint) : AbstractObject.t :=
-    let (block, instr) := pp in
-    Loc block instr.
-  
-  (* Get local variable objects *)
-  Definition get_local (P : PointsTo) (name : string) : ObjectSet.t :=
-    points_to_lookup P Locals (FKName name).
-  
-  (* Set local variable objects *)
-  Definition set_local (P : PointsTo) (name : string) (objs : ObjectSet.t) : PointsTo :=
-    upd_points_to P (ObjectSet.singleton Locals) (FKName name) objs.
-  
-  (* Get global variable objects *)
-  Definition get_global (P : PointsTo) (name : string) : ObjectSet.t :=
-    points_to_lookup P Globals (FKName name).
-  
-  (* Attribute lookup - union over all objects *)
-  Definition attr_lookup (P : PointsTo) (objs : ObjectSet.t) (attr : string) : ObjectSet.t :=
-    ObjectSet.fold (fun o acc =>
-      ObjectSet.union acc (points_to_lookup P o (FKName attr))
-    ) objs ObjectSet.empty.
-  
-  (* Index lookup with wildcard support *)
-  Definition index_lookup (P : PointsTo) (objs : ObjectSet.t) (idx : nat) : ObjectSet.t :=
-    ObjectSet.fold (fun o acc =>
-      let from_idx := points_to_lookup P o (FKPos idx) in
-      let from_star := points_to_lookup P o star in
-      ObjectSet.union acc (ObjectSet.union from_idx from_star)
-    ) objs ObjectSet.empty.
-  
-  (* ===== Transfer Functions ===== *)
-  
-  (* Move: $d := $s *)
-  Definition transfer_mov (st : State) (dst src : StackVar) : State :=
-    let S := st_stack st in
-    let objs := stack_lookup S src in
-    {| st_abstract := st_abstract st;
-       st_stack := stack_update S dst objs |}.
-  
-  (* Load constant: $d := const *)
-  Definition transfer_load_const (st : State) (dst : StackVar) (c : ConstV) : State :=
-    let S := st_stack st in
-    let obj := Imm c in
-    let T := as_types (st_abstract st) in
-    let T' := type_update T obj (object_type obj) in
-    {| st_abstract := {| as_points_to := as_points_to (st_abstract st);
-                        as_types := T' |};
-       st_stack := stack_update S dst (ObjectSet.singleton obj) |}.
-  
-  (* Load local: $d := local(x) *)
-  Definition transfer_load_local (st : State) (dst : StackVar) (name : string) : State :=
-    let P := as_points_to (st_abstract st) in
-    let S := st_stack st in
-    let objs := get_local P name in
-    {| st_abstract := st_abstract st;
-       st_stack := stack_update S dst objs |}.
-  
-  (* Load global: $d := global(x) *)
-  Definition transfer_load_global (st : State) (dst : StackVar) (name : string) : State :=
-    let P := as_points_to (st_abstract st) in
-    let S := st_stack st in
-    let objs := get_global P name in
-    {| st_abstract := st_abstract st;
-       st_stack := stack_update S dst objs |}.
-  
-  (* Set local: local(x) := $s *)
-  Definition transfer_set_local (st : State) (name : string) (src : StackVar) : State :=
-    let P := as_points_to (st_abstract st) in
-    let T := as_types (st_abstract st) in
-    let S := st_stack st in
-    let objs := stack_lookup S src in
-    let P' := set_local P name objs in
-    {| st_abstract := {| as_points_to := P'; as_types := T |};
-       st_stack := S |}.
-  
-  (* Get attribute: $d := $o.attr *)
-  Definition transfer_get_attr (st : State) (dst : StackVar) (obj_var : StackVar) (attr : string) : State :=
-    let P := as_points_to (st_abstract st) in
-    let S := st_stack st in
-    let obj_set := stack_lookup S obj_var in
-    let result := attr_lookup P obj_set attr in
-    {| st_abstract := st_abstract st;
-       st_stack := stack_update S dst result |}.
-  
-  (* Set attribute: $o.attr := $v *)
-  Definition transfer_set_attr (st : State) (obj_var : StackVar) (attr : string) (val_var : StackVar) : State :=
-    let P := as_points_to (st_abstract st) in
-    let T := as_types (st_abstract st) in
-    let S := st_stack st in
-    let targets := stack_lookup S obj_var in
-    let values := stack_lookup S val_var in
-    let P' := upd_points_to P targets (FKName attr) values in
-    {| st_abstract := {| as_points_to := P'; as_types := T |};
-       st_stack := S |}.
-  
-  (* Construct tuple: $d := tuple($e0, ..., $en) *)
-  Definition transfer_construct_tuple (st : State) (dst : StackVar) (elems : list StackVar) 
-                                      (pp : ProgramPoint) : State :=
-    let P := as_points_to (st_abstract st) in
-    let T := as_types (st_abstract st) in
-    let S := st_stack st in
-    let tup := alloc_site pp in
+      let fm := match AOMap.find o P with
+               | Some fm => fm
+               | None => FieldMap.empty _
+               end in
+      AOMap.add o (FieldMap.add f objs fm) P.
     
-    (* Wire up tuple elements at both positional and star fields *)
-    let indexed_elems := List.combine (List.seq 0 (List.length elems)) elems in
-    let P' := List.fold_left (fun P_acc pair =>
-      let (idx, elem_var) := pair in
-      let elem_objs := stack_lookup S elem_var in
-      let P1 := upd_points_to P_acc (ObjectSet.singleton tup) (FKPos idx) elem_objs in
-      upd_points_to P1 (ObjectSet.singleton tup) star elem_objs
-    ) indexed_elems P in
+    (* Strong/weak update *)
+    Definition upd_points_to (P : PointsTo) (targets : ObjectSet.t) (f : FieldKey)
+                            (new_objs : ObjectSet.t) : PointsTo :=
+      if Nat.eqb (ObjectSet.cardinal targets) 1 then
+        match ObjectSet.choose targets with
+        | Some tgt => points_to_update P tgt f new_objs
+        | None => P
+        end
+      else
+        ObjectSet.fold (fun tgt acc =>
+          let old := points_to_lookup acc tgt f in
+          points_to_update acc tgt f (ObjectSet.union old new_objs)
+        ) targets P.
     
-    (* Update type *)
-    let T' := type_update T tup (alloc_type (IConstructTuple dst elems)) in
+    (* Index lookup helper *)
+    Definition index_lookup (P : PointsTo) (objs : ObjectSet.t) (idx : nat) : ObjectSet.t :=
+      ObjectSet.fold (fun o acc =>
+        let from_pos := points_to_lookup P o (FKPos idx) in
+        let from_wild := points_to_lookup P o wildcard in
+        ObjectSet.union acc (ObjectSet.union from_pos from_wild)
+      ) objs ObjectSet.empty.
     
-    {| st_abstract := {| as_points_to := P'; as_types := T' |};
-       st_stack := stack_update S dst (ObjectSet.singleton tup) |}.
-  
-  (* Construct dict: $d := dict([(k1,v1), ...]) *)
-  Definition transfer_construct_dict (st : State) (dst : StackVar) 
-                                     (pairs : list (StackVar * StackVar)) 
-                                     (pp : ProgramPoint) : State :=
-    let P := as_points_to (st_abstract st) in
-    let T := as_types (st_abstract st) in
-    let S := st_stack st in
-    let dict := alloc_site pp in
+    (* ===== Type operations ===== *)
     
-    (* Wire up dictionary entries *)
-    let P' := List.fold_left (fun P_acc pair =>
-      let (key_var, val_var) := pair in
-      let key_objs := stack_lookup S key_var in
-      let val_objs := stack_lookup S val_var in
-      (* Check if key is a string literal *)
-      match ObjectSet.choose key_objs with
-      | Some (Imm (KString s)) =>
-          (* String key: use named field *)
-          upd_points_to P_acc (ObjectSet.singleton dict) (FKName s) val_objs
-      | _ =>
-          (* Non-string or multiple keys: use star field *)
-          upd_points_to P_acc (ObjectSet.singleton dict) star val_objs
-      end
-    ) pairs P in
+    Definition type_lookup (T : TypeMap) (o : AbstractObject.t) : TypeExpr :=
+      match AOMap.find o T with
+      | Some ty => ty
+      | None => type_bot
+      end.
     
-    (* Update type *)
-    let T' := type_update T dict (alloc_type (IConstructDict dst pairs)) in
+    Definition type_update (T : TypeMap) (o : AbstractObject.t) (ty : TypeExpr) : TypeMap :=
+      AOMap.add o (type_join (type_lookup T o) ty) T.
     
-    {| st_abstract := {| as_points_to := P'; as_types := T' |};
-       st_stack := stack_update S dst (ObjectSet.singleton dict) |}.
-  
-  (* Bind: $d := bind($f, $a, $k) - creates bound callable *)
-  Definition transfer_bind (st : State) (dst func_var args_var kwargs_var : StackVar) 
-                           (pp : ProgramPoint) : State :=
-    let P := as_points_to (st_abstract st) in
-    let T := as_types (st_abstract st) in
-    let S := st_stack st in
-    let bound := alloc_site pp in
+    Definition type_update_set (T : TypeMap) (objs : ObjectSet.t) (ty : TypeExpr) : TypeMap :=
+      ObjectSet.fold (fun o acc => type_update acc o ty) objs T.
     
-    let func_objs := stack_lookup S func_var in
-    let args_objs := stack_lookup S args_var in
-    let kwargs_objs := stack_lookup S kwargs_var in
+    Definition get_types (T : TypeMap) (objs : ObjectSet.t) : TypeExpr :=
+      ObjectSet.fold (fun o acc =>
+        type_join acc (type_lookup T o)
+      ) objs type_bot.
     
-    (* Wire up bound callable *)
-    let P1 := upd_points_to P (ObjectSet.singleton bound) (FKName "__func__") func_objs in
-    let P2 := upd_points_to P1 (ObjectSet.singleton bound) args args_objs in
-    let P' := upd_points_to P2 (ObjectSet.singleton bound) kwargs kwargs_objs in
+    (* ===== Dirty tracking ===== *)
     
-    (* Update type *)
-    let T' := type_update T bound (alloc_type (IBind dst func_var args_var kwargs_var)) in
+    Definition mark_dirty (D : DirtyMap) (o : AbstractObject.t) (f : FieldKey) : DirtyMap :=
+      let fm := match AOMap.find o D with
+               | Some fm => fm
+               | None => FieldMap.empty _
+               end in
+      AOMap.add o (FieldMap.add f true fm) D.
     
-    {| st_abstract := {| as_points_to := P'; as_types := T' |};
-       st_stack := stack_update S dst (ObjectSet.singleton bound) |}.
-  
-  (* Unpack: [$d0, ..., $dn] := unpack($s) *)
-  Definition transfer_unpack (st : State) (dsts : list StackVar) (src : StackVar) : State :=
-    let P := as_points_to (st_abstract st) in
-    let S := st_stack st in
-    let src_objs := stack_lookup S src in
+    Definition mark_dirty_set (D : DirtyMap) (objs : ObjectSet.t) (f : FieldKey) : DirtyMap :=
+      ObjectSet.fold (fun o acc => mark_dirty acc o f) objs D.
     
-    (* For each destination, collect objects from appropriate indices *)
-    let indexed_dsts := List.combine (List.seq 0 (List.length dsts)) dsts in
-    let S' := List.fold_left (fun S_acc pair =>
-      let (idx, dst) := pair in
-      let objs := index_lookup P src_objs idx in
-      stack_update S_acc dst objs
-    ) indexed_dsts S in
+    (* ===== Stack operations ===== *)
     
-    {| st_abstract := st_abstract st;
-       st_stack := S' |}.
-  
-  (* Apply effects from a function call *)
-  Definition apply_call_effects (P : PointsTo) (T : TypeMap) (S : StackEnv)
-                                (eff : EffectSummary) (func_objs args_objs : ObjectSet.t) 
-                                (pp : ProgramPoint) : (PointsTo * TypeMap * ObjectSet.t) :=
-    let result_objs := 
-      if eff.(eff_new)
-      then ObjectSet.singleton (alloc_site pp)
-      else if eff.(eff_points_to_args)
-           then ObjectSet.union args_objs (ObjectSet.singleton RetUp)
-           else ObjectSet.singleton RetUp in
+    Definition stack_lookup (S : StackEnv) (v : StackVar) : ObjectSet.t := S v.
+    Definition stack_update (S : StackEnv) (v : StackVar) (objs : ObjectSet.t) : StackEnv :=
+      fun v' => if Nat.eqb v v' then objs else S v'.
     
-    (* Apply field updates from effects *)
-    let P' := List.fold_left (fun P_acc update =>
-      let (param_idx, field) := update in
-      (* This would need to resolve which objects correspond to param_idx *)
-      (* Simplified for now *)
-      P_acc
-    ) eff.(eff_update) P in
+    (* ===== Abstract State ===== *)
     
-    (* Update type for new allocation *)
-    let T' := if eff.(eff_new)
-             then type_update T (alloc_site pp) (alloc_type (ICall 0 0))
-             else T in
+    Record AbstractState := {
+      as_points_to : PointsTo;
+      as_types : TypeMap;
+      as_dirty : DirtyMap
+    }.
     
-    (P', T', result_objs).
-  
-  (* Call: $d := call($f) *)
-  Definition transfer_call (st : State) (dst : StackVar) (func_var : StackVar) 
-                           (pp : ProgramPoint) : State :=
-    let P := as_points_to (st_abstract st) in
-    let T := as_types (st_abstract st) in
-    let S := st_stack st in
-    let func_objs := stack_lookup S func_var in
+    Record State := {
+      st_abstract : AbstractState;
+      st_stack : StackEnv
+    }.
     
-    (* Get effect summaries for all possible callables *)
-    let results := ObjectSet.fold (fun func_obj acc =>
-      match get_callable_effect func_obj with
-      | Some eff =>
-          (* Get arguments if this is a bound callable *)
-          let args_objs := 
-            if ObjectSet.mem func_obj (points_to_lookup P func_obj args)
-            then points_to_lookup P func_obj args
-            else ObjectSet.empty in
-          
-          let (P', T', res) := apply_call_effects P T S eff func_objs args_objs pp in
-          let (P_acc, T_acc, res_acc) := acc in
-          (P', T', ObjectSet.union res_acc res)
-      | None =>
-          (* Unknown callable - conservative approximation *)
-          let (P_acc, T_acc, res_acc) := acc in
-          (P_acc, T_acc, ObjectSet.add RetUp res_acc)
-      end
-    ) func_objs (P, T, ObjectSet.empty) in
+    Definition empty_abstract : AbstractState := {|
+      as_points_to := empty_points_to;
+      as_types := empty_type_map;
+      as_dirty := empty_dirty_map
+    |}.
     
-    let (P', T', result_objs) := results in
+    Definition empty_state : State := {|
+      st_abstract := empty_abstract;
+      st_stack := empty_stack
+    |}.
     
-    {| st_abstract := {| as_points_to := P'; as_types := T' |};
-       st_stack := stack_update S dst result_objs |}.
-  
-  (* Main transfer function *)
-  Definition transfer (st : State) (instr : Instruction) (pp : ProgramPoint) : State :=
-    match instr with
-    | IMov dst src => transfer_mov st dst src
-    | ILoadConst dst c => transfer_load_const st dst c
-    | ILoadLocal dst name => transfer_load_local st dst name
-    | ILoadGlobal dst name => transfer_load_global st dst name
-    | ISetLocal name src => transfer_set_local st name src
-    | IGetAttr dst obj attr => transfer_get_attr st dst obj attr
-    | ISetAttr obj attr val => transfer_set_attr st obj attr val
-    | IConstructTuple dst elems => transfer_construct_tuple st dst elems pp
-    | IConstructDict dst pairs => transfer_construct_dict st dst pairs pp
-    | IBind dst f a k => transfer_bind st dst f a k pp
-    | IUnpack dsts src => transfer_unpack st dsts src
-    | ICall dst func => transfer_call st dst func pp
-    | ILookupDunderUnary dst _ _ => st  (* Pure - no heap change *)
-    | ILookupDunderBinary dst _ _ _ => st  (* Pure - no heap change *)
-    | IResolveOverload dst _ _ _ => st  (* Pure - no heap change *)
-    | IAssumeValue _ _ => st  (* No state change *)
-    | IExit => st  (* No state change *)
-    end.
-  
-  (* ===== Reachability Analysis ===== *)
-  
-  (* Collect all objects reachable from a single object *)
-  Definition reachable_from_object (P : PointsTo) (o : AbstractObject.t) : ObjectSet.t :=
-    match AOMap.find o P with
-    | Some fm =>
-        AFMap.fold (fun _ objs acc =>
-          ObjectSet.union acc objs
-        ) fm ObjectSet.empty
-    | None => ObjectSet.empty
-    end.
-  
-  (* Fixed-point computation of reachability *)
-  Fixpoint compute_reachable (P : PointsTo) (worklist : ObjectSet.t) 
-                             (visited : ObjectSet.t) (fuel : nat) : ObjectSet.t :=
-    match fuel with
-    | 0 => visited
-    | S fuel' =>
-        if ObjectSet.is_empty worklist
-        then visited
+    (* ===== Location helpers ===== *)
+    
+    Definition alloc_site (pp : ProgramPoint) : AbstractObject.t :=
+      let '(b, i) := pp in Location b i.
+    
+    Definition get_local (P : PointsTo) (name : string) : ObjectSet.t :=
+      points_to_lookup P Locals (FKName name).
+    
+    Definition set_local (P : PointsTo) (name : string) (objs : ObjectSet.t) : PointsTo :=
+      upd_points_to P (ObjectSet.singleton Locals) (FKName name) objs.
+    
+    Definition get_global (P : PointsTo) (name : string) : ObjectSet.t :=
+      points_to_lookup P Globals (FKName name).
+    
+    (* ===== Expression Evaluation ===== *)
+    
+    Definition eval_const (c : ConstV) : (ObjectSet.t * TypeExpr) :=
+      let ty := literal_type c in
+      (immutable_const c, ty).
+    
+    (* Attribute lookup with bound method creation *)
+    Definition eval_attribute (st : AbstractState) (var_objs : ObjectSet.t) 
+                             (attr : string) (pp : ProgramPoint) 
+                             : (AbstractState * ObjectSet.t * TypeExpr) :=
+      let var_type := get_types (as_types st) var_objs in
+      let attr_type := subscr var_type attr in
+      
+      let result_type := 
+        if is_property attr_type then
+          get_return attr_type
         else
-          match ObjectSet.choose worklist with
-          | Some o =>
-              let worklist' := ObjectSet.remove o worklist in
-              if ObjectSet.mem o visited
-              then compute_reachable P worklist' visited fuel'
-              else
-                let visited' := ObjectSet.add o visited in
-                let new_objs := reachable_from_object P o in
-                let worklist'' := ObjectSet.union worklist' new_objs in
-                compute_reachable P worklist'' visited' fuel'
-          | None => visited
-          end
-    end.
-  
-  (* Get root objects from live variables *)
-  Definition get_roots (P : PointsTo) (live : list string) : ObjectSet.t :=
-    List.fold_left (fun acc var =>
-      ObjectSet.union acc (get_local P var)
-    ) live ObjectSet.empty.
-  
-  (* Abstract GC: restrict state to reachable objects *)
-  Definition abstract_gc (st : AbstractState) (live : list string) : AbstractState :=
-    let P := as_points_to st in
-    let T := as_types st in
-    let roots := get_roots P live in
-    let reachable := compute_reachable P roots ObjectSet.empty 1000 in
+          attr_type in
+      
+      let (st', result_objs) :=
+        if type_is_immutable result_type then
+          (st, immutable_type result_type)
+        else if is_bound_method attr_type then
+          let bm := alloc_site pp in
+          (* functions behind this attribute on each receiver *)
+          let func_objs :=
+            ObjectSet.fold (fun o acc =>
+              ObjectSet.union acc (points_to_lookup (as_points_to st) o (FKName attr))
+            ) var_objs ObjectSet.empty in
+          let P0 := upd_points_to (as_points_to st) (ObjectSet.singleton bm) self_field var_objs in
+          let P1 := upd_points_to P0 (ObjectSet.singleton bm) func_field func_objs in
+          let T' := type_update (as_types st) bm attr_type in
+          ({| as_points_to := P1; as_types := T'; as_dirty := as_dirty st |},
+           ObjectSet.singleton bm)
+        else if any_new attr_type && all_new attr_type then
+          (* Property that always allocates *)
+          let new_obj := alloc_site pp in
+          let T' := type_update (as_types st) new_obj result_type in
+          ({| as_points_to := as_points_to st; as_types := T'; as_dirty := as_dirty st |},
+           ObjectSet.singleton new_obj)
+        else
+          (* Read from field *)
+          let field_objs := ObjectSet.fold (fun o acc =>
+            ObjectSet.union acc (points_to_lookup (as_points_to st) o (FKName attr))
+          ) var_objs ObjectSet.empty in
+          if any_new attr_type then
+            let new_obj := alloc_site pp in
+            let T' := type_update (as_types st) new_obj result_type in
+            ({| as_points_to := as_points_to st; as_types := T'; as_dirty := as_dirty st |},
+             ObjectSet.union field_objs (ObjectSet.singleton new_obj))
+          else
+            (st, field_objs) in
+      
+      (st', result_objs, result_type).
+      
+    (* Collect values behind wildcard of a container set (tuples/dicts). *)
+    Definition collect_wild_values (P:PointsTo) (containers:ObjectSet.t) : ObjectSet.t :=
+      ObjectSet.fold (fun o acc => ObjectSet.union acc (points_to_lookup P o wildcard))
+                     containers ObjectSet.empty.
     
-    (* Filter points-to map *)
-    let P' := AOMap.fold (fun o fm acc =>
-      if ObjectSet.mem o reachable
-      then AOMap.add o fm acc
-      else acc
-    ) P empty_points_to in
+    (* Read bound-call state off a callee object *)
+    Definition bound_args_tuples (P:PointsTo) (callee:ObjectSet.t) : ObjectSet.t :=
+      ObjectSet.fold (fun f acc => ObjectSet.union acc (points_to_lookup P f args_field))
+                     callee ObjectSet.empty.
     
-    (* Filter type map *)
-    let T' := AOMap.fold (fun o ty acc =>
-      if ObjectSet.mem o reachable
-      then AOMap.add o ty acc
-      else acc
-    ) T empty_type_map in
+    Definition bound_kwargs_dicts (P:PointsTo) (callee:ObjectSet.t) : ObjectSet.t :=
+      ObjectSet.fold (fun f acc => ObjectSet.union acc (points_to_lookup P f kwargs_field))
+                     callee ObjectSet.empty.
     
-    {| as_points_to := P'; as_types := T' |}.
-  
-  (* ===== Lattice Operations ===== *)
-  
-  (* Join points-to maps *)
-  Definition join_points_to (P1 P2 : PointsTo) : PointsTo :=
-    AOMap.fold (fun o fm1 acc =>
-      match AOMap.find o P2 with
-      | Some fm2 =>
-          (* Join field maps *)
-          let fm_joined := AFMap.fold (fun f objs1 fm_acc =>
-            match AFMap.find f fm2 with
-            | Some objs2 => AFMap.add f (ObjectSet.union objs1 objs2) fm_acc
-            | None => AFMap.add f objs1 fm_acc
-            end
-          ) fm1 fm2 in
-          AOMap.add o fm_joined acc
-      | None => AOMap.add o fm1 acc
-      end
-    ) P1 P2.
-  
-  (* Join type maps *)
-  Definition join_type_maps (T1 T2 : TypeMap) : TypeMap :=
-    AOMap.fold (fun o ty1 acc =>
-      match AOMap.find o T2 with
-      | Some ty2 => AOMap.add o (type_join ty1 ty2) acc
-      | None => AOMap.add o ty1 acc
-      end
-    ) T1 T2.
-  
-  (* Join abstract states *)
-  Definition join_states (st1 st2 : AbstractState) : AbstractState := {|
-    as_points_to := join_points_to (as_points_to st1) (as_points_to st2);
-    as_types := join_type_maps (as_types st1) (as_types st2);
-  |}.
-  
-  (* Order on abstract states *)
-  Definition state_leq (st1 st2 : AbstractState) : Prop :=
-    (forall o f, ObjectSet.Subset 
-      (points_to_lookup (as_points_to st1) o f)
-      (points_to_lookup (as_points_to st2) o f)) /\
-    (forall o, type_leq (type_lookup (as_types st1) o) 
-                        (type_lookup (as_types st2) o) = true).
-  
-  (* ===== Key Properties (Admitted) ===== *)
-  
-  (* Join is least upper bound *)
-  Lemma join_is_lub :
-    forall st1 st2 st',
-    state_leq st1 st' ->
-    state_leq st2 st' ->
-    state_leq (join_states st1 st2) st'.
-  Proof.
-    Admitted.
-  
-  (* Transfer functions are monotonic *)
-  Lemma transfer_monotonic :
-    forall st1 st2 instr pp,
-    state_leq st1 st2 ->
-    state_leq 
-      (st_abstract (transfer {| st_abstract := st1; st_stack := empty_stack |} instr pp))
-      (st_abstract (transfer {| st_abstract := st2; st_stack := empty_stack |} instr pp)).
-  Proof.
-    Admitted.
-  
-  (* GC preserves soundness *)
-  Lemma gc_sound :
-    forall st live st',
-    st' = abstract_gc st live ->
-    (* For all reachable objects, their points-to info is preserved *)
-    True.
-  Proof.
-    Admitted.
-  
+    Definition bound_self (P:PointsTo) (callee:ObjectSet.t) : ObjectSet.t :=
+      ObjectSet.fold (fun f acc => ObjectSet.union acc (points_to_lookup P f self_field))
+                     callee ObjectSet.empty.
+                     
+    (* ---------- Joins (points-to / types / dirty) ---------- *)
+    
+    Definition join_fieldmaps (fm1 fm2 : FieldMap.t ObjectSet.t) : FieldMap.t ObjectSet.t :=
+      FieldMap.fold (fun k objs acc =>
+        let old := match FieldMap.find k acc with | Some o => o | None => ObjectSet.empty end in
+        FieldMap.add k (ObjectSet.union old objs) acc
+      ) fm2 fm1.
+    
+    Definition join_points_to (P1 P2 : PointsTo) : PointsTo :=
+      AOMap.fold (fun o fm acc =>
+        let old := match AOMap.find o acc with | Some fm0 => fm0 | None => FieldMap.empty _ end in
+        AOMap.add o (join_fieldmaps old fm) acc
+      ) P2 P1.
+    
+    Definition join_type_maps (T1 T2 : TypeMap) : TypeMap :=
+      AOMap.fold (fun o ty acc =>
+        let old := match AOMap.find o acc with | Some ty0 => ty0 | None => type_bot end in
+        AOMap.add o (type_join old ty) acc
+      ) T2 T1.
+    
+    Definition join_dirty_field (b1 b2 : bool) := orb b1 b2.
+    
+    Definition join_dirty_maps (D1 D2 : DirtyMap) : DirtyMap :=
+      AOMap.fold (fun o fm2 acc =>
+        let fm1 := match AOMap.find o acc with | Some fm => fm | None => FieldMap.empty _ end in
+        let fm' :=
+          FieldMap.fold (fun k b accfm =>
+            let old := match FieldMap.find k accfm with | Some bb => bb | None => false end in
+            FieldMap.add k (join_dirty_field old b) accfm
+          ) fm2 fm1
+        in AOMap.add o fm' acc
+      ) D2 D1.
+    
+    Definition join_abs (s1 s2 : AbstractState) : AbstractState :=
+      {| as_points_to := join_points_to (as_points_to s1) (as_points_to s2);
+         as_types     := join_type_maps (as_types s1)     (as_types s2);
+         as_dirty     := join_dirty_maps (as_dirty s1)    (as_dirty s2) |}.
+    
+    (* ---------- Per-callee evaluator ---------- *)
+    
+    (* One callee object -> apply bound-call semantics and side-effect summary. *)
+    Definition eval_call_single (st : AbstractState) (callee : AbstractObject.t) (pp : ProgramPoint)
+      : (AbstractState * ObjectSet.t * TypeExpr) :=
+      let P := as_points_to st in
+      let T := as_types st in
+      let callee_set := ObjectSet.singleton callee in
+    
+      (* Read bound state from the callee object *)
+      let args_tups := bound_args_tuples P callee_set in
+      let kwargs_ds := bound_kwargs_dicts P callee_set in
+      let self_objs := bound_self P callee_set in
+    
+      (* Argument typing for TS.partial (coarse but sound) *)
+      let pos_vals := collect_wild_values P args_tups in
+      let kw_vals  := collect_wild_values P kwargs_ds in
+      let arg_types := [ type_join (get_types T pos_vals) (get_types T kw_vals) ] in
+    
+      (* Callee type and effects *)
+      let func_ty   := type_lookup T callee in
+      let applied   := partial func_ty arg_types in
+      let effect    := get_side_effect applied in
+      let ret_ty    := get_return applied in
+    
+      (* Result objects *)
+      let res_objs :=
+        if type_is_immutable ret_ty then immutable_type ret_ty
+        else if se_new effect then ObjectSet.singleton (alloc_site pp)
+        else if se_points_to_args effect then ObjectSet.union pos_vals kw_vals
+        else ObjectSet.empty in
+    
+      (* Optional self update/mutation *)
+      let st' :=
+        match se_update effect with
+        | Some up_ty =>
+            let T' := ObjectSet.fold (fun o acc => type_update acc o up_ty) self_objs T in
+            let D' := mark_dirty_set (as_dirty st) self_objs wildcard in
+            let P' :=
+              match se_update_indices effect with
+              | [] => P
+              | idxs =>
+                  List.fold_left (fun acc idx =>
+                     let param_objs := index_lookup P args_tups idx in
+                     upd_points_to acc self_objs wildcard param_objs
+                  ) idxs P
+              end in
+            {| as_points_to := P'; as_types := T'; as_dirty := D' |}
+        | None => st
+        end in
+    
+      (* Type fresh allocs and wire aliasing into them when requested *)
+      let st'' :=
+        if se_new effect then
+          let T'' := type_update (as_types st') (alloc_site pp) ret_ty in
+          {| as_points_to := as_points_to st'; as_types := T''; as_dirty := as_dirty st' |}
+        else st' in
+      let st''' :=
+        if se_new effect && se_points_to_args effect then
+          let ali := ObjectSet.union pos_vals kw_vals in
+          let P'' := upd_points_to (as_points_to st'') (ObjectSet.singleton (alloc_site pp)) wildcard ali in
+          {| as_points_to := P''; as_types := as_types st''; as_dirty := as_dirty st'' |}
+        else st'' in
+    
+      (st''', res_objs, ret_ty).
+    
+    (* ---------- Multi-callee aggregator ---------- *)
+    
+    (* Possibly-many callees -> fold eval_call_single and join states/types/objects/types. *)
+    Definition eval_call (st : AbstractState) (func_objs : ObjectSet.t) (pp : ProgramPoint)
+      : (AbstractState * ObjectSet.t * TypeExpr) :=
+      ObjectSet.fold
+        (fun f acc =>
+           let '(acc_st, acc_objs, acc_ty) := acc in
+           let '(one_st, one_objs, one_ty) := eval_call_single acc_st f pp in
+           (one_st, ObjectSet.union acc_objs one_objs, type_join acc_ty one_ty))
+        func_objs
+        (st, ObjectSet.empty, type_bot).
+    
+    
+    (* ===== Transfer Functions ===== *)
+    
+    Definition transfer_load_const (st : State) (dst : StackVar) (c : ConstV) : State :=
+      let (objs, ty) := eval_const c in
+      let T' := type_update_set (as_types (st_abstract st)) objs ty in
+      {| st_abstract := {| as_points_to := as_points_to (st_abstract st);
+                          as_types := T';
+                          as_dirty := as_dirty (st_abstract st) |};
+         st_stack := stack_update (st_stack st) dst objs |}.
+    
+    Definition transfer_load_local (st : State) (dst : StackVar) (name : string) : State :=
+      let objs := get_local (as_points_to (st_abstract st)) name in
+      {| st_abstract := st_abstract st;
+         st_stack := stack_update (st_stack st) dst objs |}.
+    
+    Definition transfer_load_global (st : State) (dst : StackVar) (name : string) : State :=
+      let objs := get_global (as_points_to (st_abstract st)) name in
+      {| st_abstract := st_abstract st;
+         st_stack := stack_update (st_stack st) dst objs |}.
+    
+    Definition transfer_set_local (st : State) (name : string) (src : StackVar) : State :=
+      let objs := stack_lookup (st_stack st) src in
+      let P' := set_local (as_points_to (st_abstract st)) name objs in
+      {| st_abstract := {| as_points_to := P';
+                          as_types := as_types (st_abstract st);
+                          as_dirty := as_dirty (st_abstract st) |};
+         st_stack := st_stack st |}.
+    
+    Definition transfer_get_attr (st : State) (dst : StackVar) (obj : StackVar) 
+                                 (attr : string) (pp : ProgramPoint) : State :=
+      let obj_set := stack_lookup (st_stack st) obj in
+      let (st', result_objs, result_type) := eval_attribute (st_abstract st) obj_set attr pp in
+      let T' := type_update_set (as_types st') result_objs result_type in
+      {| st_abstract := {| as_points_to := as_points_to st';
+                          as_types := T';
+                          as_dirty := as_dirty st' |};
+         st_stack := stack_update (st_stack st) dst result_objs |}.
+    
+    Definition transfer_set_attr (st : State) (obj : StackVar) (attr : string) 
+                                 (val : StackVar) : State :=
+      let targets := stack_lookup (st_stack st) obj in
+      let values := stack_lookup (st_stack st) val in
+      let P' := upd_points_to (as_points_to (st_abstract st)) targets (FKName attr) values in
+      let D' := mark_dirty_set (as_dirty (st_abstract st)) targets (FKName attr) in
+      {| st_abstract := {| as_points_to := P';
+                          as_types := as_types (st_abstract st);
+                          as_dirty := D' |};
+         st_stack := st_stack st |}.
+    
+    Definition transfer_construct_tuple (st : State) (dst : StackVar) (elems : list StackVar)
+                                       (pp : ProgramPoint) : State :=
+      let tup := alloc_site pp in
+      let indexed_elems := List.combine (List.seq 0 (List.length elems)) elems in
+      let P' := List.fold_left (fun acc pair =>
+        let (idx, elem) := pair in
+        let elem_objs := stack_lookup (st_stack st) elem in
+        let P1 := upd_points_to acc (ObjectSet.singleton tup) (FKPos idx) elem_objs in
+        upd_points_to P1 (ObjectSet.singleton tup) wildcard elem_objs
+      ) indexed_elems (as_points_to (st_abstract st)) in
+      let T' := type_update (as_types (st_abstract st)) tup 
+                           (get_return make_tuple_constructor) in
+      {| st_abstract := {| as_points_to := P';
+                          as_types := T';
+                          as_dirty := as_dirty (st_abstract st) |};
+         st_stack := stack_update (st_stack st) dst (ObjectSet.singleton tup) |}.
+    
+    Definition transfer_construct_dict (st : State) (dst : StackVar) 
+                                      (pairs : list (StackVar * StackVar))
+                                      (pp : ProgramPoint) : State :=
+      let dict := alloc_site pp in
+      let P' := List.fold_left (fun acc pair =>
+        let (key_var, val_var) := pair in
+        let key_objs := stack_lookup (st_stack st) key_var in
+        let val_objs := stack_lookup (st_stack st) val_var in
+        (* Check if key is a string literal *)
+        let P0 := upd_points_to acc (ObjectSet.singleton dict) wildcard val_objs in
+        match ObjectSet.choose key_objs with
+        | Some (ImmConst (KString s))
+          => if Nat.eqb (ObjectSet.cardinal key_objs) 1
+             then upd_points_to P0 (ObjectSet.singleton dict) (FKName s) val_objs
+             else P0
+        | _ => P0
+        end
+      ) pairs (as_points_to (st_abstract st)) in
+      let T' := type_update (as_types (st_abstract st)) dict 
+                           (get_return make_dict_constructor) in
+      {| st_abstract := {| as_points_to := P';
+                          as_types := T';
+                          as_dirty := as_dirty (st_abstract st) |};
+         st_stack := stack_update (st_stack st) dst (ObjectSet.singleton dict) |}.
+    
+    Definition transfer_bind (st : State) (dst func_var args_var kwargs_var : StackVar)
+                            (pp : ProgramPoint) : State :=
+      let bound := alloc_site pp in
+      let func_objs := stack_lookup (st_stack st) func_var in
+      let args_objs := stack_lookup (st_stack st) args_var in
+      let kwargs_objs := stack_lookup (st_stack st) kwargs_var in
+      
+      (* Wire bound callable structure *)
+      let P1 := upd_points_to (as_points_to (st_abstract st)) 
+                              (ObjectSet.singleton bound) func_field func_objs in
+      let P2 := upd_points_to P1 (ObjectSet.singleton bound) args_field args_objs in
+      let P3 := upd_points_to P2 (ObjectSet.singleton bound) kwargs_field kwargs_objs in
+      
+      (* Extract self from args[0] *)
+      let self_objs := index_lookup P3 args_objs 0 in
+      let P4 := if ObjectSet.is_empty self_objs then P3
+               else upd_points_to P3 (ObjectSet.singleton bound) self_field self_objs in
+      
+      (* Type the bound object *)
+      let T' := type_update (as_types (st_abstract st)) bound 
+                           (get_types (as_types (st_abstract st)) func_objs) in
+      
+      {| st_abstract := {| as_points_to := P4;
+                          as_types := T';
+                          as_dirty := as_dirty (st_abstract st) |};
+         st_stack := stack_update (st_stack st) dst (ObjectSet.singleton bound) |}.
+    
+    Definition transfer_unpack (st : State) (dsts : list StackVar) (src : StackVar) : State :=
+      let src_objs := stack_lookup (st_stack st) src in
+      let indexed_dsts := List.combine (List.seq 0 (List.length dsts)) dsts in
+      let S' := List.fold_left (fun acc pair =>
+        let (idx, dst) := pair in
+        let objs := index_lookup (as_points_to (st_abstract st)) src_objs idx in
+        stack_update acc dst objs
+      ) indexed_dsts (st_stack st) in
+      {| st_abstract := st_abstract st;
+         st_stack := S' |}.
+    
+    Definition transfer_call (st : State) (dst : StackVar) (func : StackVar) (pp : ProgramPoint) : State :=
+      let func_objs := stack_lookup (st_stack st) func in
+      let (st', result_objs, result_type) := eval_call (st_abstract st) func_objs pp in
+      let T' := type_update_set (as_types st') result_objs result_type in
+      {| st_abstract := {| as_points_to := as_points_to st';
+                          as_types := T';
+                          as_dirty := as_dirty st' |};
+         st_stack := stack_update (st_stack st) dst result_objs |}.
+    
+    (* Main transfer dispatcher *)
+    Definition transfer (st : State) (instr : Instruction) (pp : ProgramPoint) : State :=
+      match instr with
+      | IMov d s => 
+          {| st_abstract := st_abstract st;
+             st_stack := stack_update (st_stack st) d (stack_lookup (st_stack st) s) |}
+      | ILoadConst d c => transfer_load_const st d c
+      | ILoadLocal d x => transfer_load_local st d x
+      | ILoadGlobal d x => transfer_load_global st d x
+      | ISetLocal x s => transfer_set_local st x s
+      | IGetAttr d o a => transfer_get_attr st d o a pp
+      | ISetAttr o a v => transfer_set_attr st o a v
+      | IConstructTuple d xs => transfer_construct_tuple st d xs pp
+      | IConstructDict d kvs => transfer_construct_dict st d kvs pp
+      | IBind d f a k => transfer_bind st d f a k pp
+      | IUnpack ds s => transfer_unpack st ds s
+      | ICall d f => transfer_call st d f pp
+      (* Pure lookups - mark as immutable *)
+      | ILookupDunderUnary d _ _ | ILookupDunderBinary d _ _ _ | ILookupOverload d _ _ _ =>
+          let imm := immutable_type type_bot in
+          {| st_abstract := st_abstract st;
+             st_stack := stack_update (st_stack st) d imm |}
+      | IAssumeValue _ _ => st
+      | IExit => st
+      end.
+    
+  End Analysis.
+
 End PointerAnalysis.
